Test/git-issues/git-issue-1604.dfy
@@ -42,24 +42,35 @@ predicate method isSetOfCompilableEvenCells(s: set<CompilableEvenCell>) {
   forall c :: c in s ==> returnsOneIfCompilableEvenCell(c) == 1
 }
 
-function method isGhostEvenCell(c: Cell): (r: bool)
+function method isEvenCell(c: Cell): (r: bool)
 {
   c.x == 0
 }
 
+predicate method {:opaque} isMod2(c: Cell)
+  ensures c.x % 2 == 0 <==> isMod2(c)
+ {
+  c.x % 2 == 0
+}
+
+
 method Main() {
   var x: set<Cell> := getOriginalSet();
-
   var b := true;
-  // This line should work because c is assigned the type GhostEvenCell early in the process, so it can be assigned the type Cell in the rangee
-  // and thus resolution does not fail.
+
+  // This line should work because c should be of type Cell as the constraint is not compilable
   // Since it figures out the type of c later, it will be resolved as a "GhostEvenCell" everywhere.
-  b := b && isSetOfGhostEvenCells(set c: GhostEvenCell | c in x && c.x % 4 == 0 :: c);
+  b := b && isSetOfGhostEvenCells(set c | c in x && isEvenCell(c) && ghostEvenCellIsOneOrMore(c) :: c);
 
   // This line should work because c is assigned the type GhostEvenCell early in the process, so it can be assigned the type Cell in the rangee
   // and thus resolution does not fail.
   // Since it figures out the type of c later, it will be resolved as a "GhostEvenCell" everywhere.
-  b := b && isSetOfGhostEvenCells(set c: GhostEvenCell | c in x && isGhostEvenCell(c) && ghostEvenCellIsOneOrMore(c) :: c);
+  b := b && isSetOfGhostEvenCells(set c: GhostEvenCell | c in x && isMod2(c) :: c);
+
+  // This line should work because c is assigned the type GhostEvenCell early in the process, so it can be assigned the type Cell in the rangee
+  // and thus resolution does not fail.
+  // Since it figures out the type of c later, it will be resolved as a "GhostEvenCell" everywhere.
+  b := b && isSetOfGhostEvenCells(set c: GhostEvenCell | c in x && isEvenCell(c) && ghostEvenCellIsOneOrMore(c) :: c);
 
   // This line should work because the output type constraint can be proven
   // c should be assigned the type Cell in the range expression, but GhostEvenCell in the term expression
@@ -86,7 +97,6 @@ method Main() {
   // This line works because the test is added right after the assignment of c, although it is evaluated twice.
   b := b && isSetOfCompilableEvenCells(set c: CompilableEvenCell | c in x && compiledEvenCellIsOneOrMore(c) && c.x % 2 == 0);
 
-
   // This line should work although the result is not of type set<GhostEvenCell>
   b := b && isSetOfCompilableEvenCells(set c | c in x && c.x % 2 == 0);
 
@@ -102,7 +112,14 @@ method Main() {
     // This line should work because the precondition of compiledEvenCellIsOneOrMore is met although it's executed twice
   b := b && isSetOfCompilableEvenCells(set c | c in x && c.x % 2 == 0 && compiledEvenCellIsOneOrMore(c));
 
+  var x2: set<GhostEvenCell> := set c: GhostEvenCell | c in x && c.x % 2 == 0;
+  // This line should work because c is taken from a set of GhostEvenCell already
+  b := b && isSetOfGhostEvenCells(set c: GhostEvenCell | c in x2 :: c);
+
+// This line should work because c is taken from a set of GhostEvenCell already
+  b := b && isSetOfGhostEvenCells(set c: GhostEvenCell | c in x2 && ghostEvenCellIsOneOrMore(c) :: c);
   assert b;
+
   print if b then "ok" else "error";
 }
 
